src/RewriterRulesGood.v
@@ -44,150 +44,10 @@ Module Compilers.
   Module Import RewriteRules.
     Import Rewriter.Compilers.RewriteRules.
 
-    Lemma nbe_rewrite_head_eq : @nbe_rewrite_head = @nbe_rewrite_head0.
-    Proof. reflexivity. Qed.
-
-    Lemma fancy_rewrite_head_eq
-      : (fun var do_again => @fancy_rewrite_head var)
-        = @fancy_rewrite_head0.
-    Proof. reflexivity. Qed.
-
-    Lemma arith_rewrite_head_eq max_const_val : (fun var do_again => @arith_rewrite_head max_const_val var) = (fun var => @arith_rewrite_head0 var max_const_val).
-    Proof. reflexivity. Qed.
-
-    Lemma fancy_with_casts_rewrite_head_eq invert_low invert_high value_range flag_range
-      : (fun var do_again => @fancy_with_casts_rewrite_head invert_low invert_high value_range flag_range var)
-        = (fun var => @fancy_with_casts_rewrite_head0 var invert_low invert_high value_range flag_range).
-    Proof. reflexivity. Qed.
-
-    Lemma arith_with_casts_rewrite_head_eq : @arith_with_casts_rewrite_head = @arith_with_casts_rewrite_head0.
-    Proof. reflexivity. Qed.
-
-    Lemma strip_literal_casts_rewrite_head_eq : (fun var do_again => @strip_literal_casts_rewrite_head var) = @strip_literal_casts_rewrite_head0.
-    Proof. reflexivity. Qed.
-
-    Lemma nbe_all_rewrite_rules_eq : @nbe_all_rewrite_rules = @nbe_rewrite_rules.
-    Proof. reflexivity. Qed.
-
-    Lemma fancy_all_rewrite_rules_eq : @fancy_all_rewrite_rules = @fancy_rewrite_rules.
-    Proof. reflexivity. Qed.
-
-    Lemma arith_all_rewrite_rules_eq : @arith_all_rewrite_rules = @arith_rewrite_rules.
-    Proof. reflexivity. Qed.
-
-    Lemma fancy_with_casts_all_rewrite_rules_eq : @fancy_with_casts_all_rewrite_rules = @fancy_with_casts_rewrite_rules.
-    Proof. reflexivity. Qed.
-
-    Lemma arith_with_casts_all_rewrite_rules_eq : @arith_with_casts_all_rewrite_rules = @arith_with_casts_rewrite_rules.
-    Proof. reflexivity. Qed.
-
-    Lemma strip_literal_casts_all_rewrite_rules_eq : @strip_literal_casts_all_rewrite_rules = @strip_literal_casts_rewrite_rules.
-    Proof. reflexivity. Qed.
-
     Section good.
       Context {var1 var2 : type -> Type}.
 
       Local Notation rewrite_rules_goodT := (@Compile.rewrite_rules_goodT ident pattern.ident (@pattern.ident.arg_types) var1 var2).
-
-      Lemma wf_rlist_rect_gen
-            {ivar1 ivar2 A P}
-            Q
-            N1 N2 C1 C2 ls1 ls2 G
-            (Hwf : expr.wf G ls1 ls2)
-            (HN : UnderLets.wf Q G N1 N2)
-            (HC : forall G' x xs y ys rec1 rec2,
-                (exists seg, G' = (seg ++ G)%list)
-                -> expr.wf G x y
-                -> expr.wf G (reify_list xs) (reify_list ys)
-                -> Q G' rec1 rec2
-                -> UnderLets.wf Q G' (C1 x xs rec1) (C2 y ys rec2))
-        : option_eq (UnderLets.wf Q G)
-                    (@rlist_rect var1 A P ivar1 N1 C1 ls1)
-                    (@rlist_rect var2 A P ivar2 N2 C2 ls2).
-      Proof using Type.
-        cbv [rlist_rect].
-        cbv [Compile.option_bind' Option.bind].
-        break_innermost_match.
-        all: repeat first [ match goal with
-                            | [ H : invert_expr.reflect_list ?v = Some _, H' : invert_expr.reflect_list ?v' = None |- _ ]
-                              => first [ erewrite <- expr.wf_reflect_list in H' by eassumption
-                                      | erewrite -> expr.wf_reflect_list in H' by eassumption ];
-                                exfalso; clear -H H'; congruence
-                            | [ |- UnderLets.wf _ _ _ _ ] => constructor
-                            end
-                          | progress expr.invert_subst
-                          | progress cbn [sequence_return option_eq]
-                          | assumption
-                          | reflexivity
-                          | apply @UnderLets.wf_splice with (P:=fun G' => expr.wf G')
-                          | progress intros ].
-        lazymatch goal with
-        | [ H : expr.wf _ (reify_list ?l) (reify_list ?l') |- _ ]
-          => revert dependent l'; intro l2; revert dependent l; intro l1
-        end.
-        revert l2; induction l1 as [|l1 ls1 IHls1], l2; cbn [list_rect];
-          rewrite ?expr.reify_list_cons, ?expr.reify_list_nil;
-          intros; expr.inversion_wf_constr; [ assumption | ].
-        all: repeat first [ match goal with
-                            | [ H : invert_expr.reflect_list ?v = Some _, H' : invert_expr.reflect_list ?v' = None |- _ ]
-                              => first [ erewrite <- expr.wf_reflect_list in H' by eassumption
-                                      | erewrite -> expr.wf_reflect_list in H' by eassumption ];
-                                exfalso; clear -H H'; congruence
-                            | [ |- UnderLets.wf _ _ _ _ ] => constructor
-                            end
-                          | progress expr.invert_subst
-                          | progress cbn [sequence_return option_eq]
-                          | assumption
-                          | reflexivity
-                          | solve [ auto ]
-                          | progress subst
-                          | apply @UnderLets.wf_splice with (P:=Q)
-                          | progress intros
-                          | wf_safe_t_step
-                          | progress type.inversion_type
-                          | progress expr.inversion_wf_constr ].
-      Qed.
-      Lemma wf_rlist_rect {A P}
-            N1 N2 C1 C2 ls1 ls2 G
-            (Hwf : expr.wf G ls1 ls2)
-            (HN : UnderLets.wf (fun G' => expr.wf G') G N1 N2)
-            (HC : forall G' x xs y ys rec1 rec2,
-                (exists seg, G' = (seg ++ G)%list)
-                -> expr.wf G x y
-                -> expr.wf G (reify_list xs) (reify_list ys)
-                -> expr.wf G' rec1 rec2
-                -> UnderLets.wf (fun G'' => expr.wf G'') G' (C1 x xs rec1) (C2 y ys rec2))
-        : option_eq (UnderLets.wf (fun G' => expr.wf G') G)
-                    (@rlist_rect var1 A P var1 N1 C1 ls1)
-                    (@rlist_rect var2 A P var2 N2 C2 ls2).
-      Proof using Type. apply wf_rlist_rect_gen; assumption. Qed.
-      Lemma wf_rlist_rectv {A P}
-            N1 N2 C1 C2 ls1 ls2 G
-            (Hwf : expr.wf G ls1 ls2)
-            (HN : UnderLets.wf (fun G' v1 v2
-                                => exists G'',
-                                    (forall t' v1' v2', List.In (existT _ t' (v1', v2')) G'' -> Compile.wf_value G' v1' v2')
-                                    /\ expr.wf G'' v1 v2) G N1 N2)
-            (HC : forall G' x xs y ys rec1 rec2,
-                (exists seg, G' = (seg ++ G)%list)
-                -> expr.wf G x y
-                -> expr.wf G (reify_list xs) (reify_list ys)
-                -> (exists G'', (forall t' v1' v2', List.In (existT _ t' (v1', v2')) G'' -> Compile.wf_value G' v1' v2')
-                                /\ expr.wf G'' rec1 rec2)
-                -> UnderLets.wf (fun G' v1 v2
-                                 => exists G'',
-                                     (forall t' v1' v2', List.In (existT _ t' (v1', v2')) G'' -> Compile.wf_value G' v1' v2')
-                                     /\ expr.wf G'' v1 v2)
-                                G' (C1 x xs rec1) (C2 y ys rec2))
-        : option_eq (UnderLets.wf
-                       (fun G' v1 v2
-                        => exists G'',
-                            (forall t' v1' v2', List.In (existT _ t' (v1', v2')) G'' -> Compile.wf_value G' v1' v2')
-                            /\ expr.wf G'' v1 v2)
-                       G)
-                    (@rlist_rect var1 A P (@Compile.value _ ident var1) N1 C1 ls1)
-                    (@rlist_rect var2 A P (@Compile.value _ ident var2) N2 C2 ls2).
-      Proof using Type. apply wf_rlist_rect_gen; assumption. Qed.
 
       Lemma wf_list_rect {T A}
             G N1 N2 C1 C2 ls1 ls2
@@ -222,22 +82,29 @@ Module Compilers.
             (nat_rect (fun _ => @Compile.value_with_lets base.type ident var2 A) O2 S2 n).
       Proof. induction n; cbn [nat_rect]; try eapply HS; eauto using (ex_intro _ nil). Qed.
 
+      Global Strategy -100 [rewrite_rules Compile.rewrite_rules_goodT_curried_cps].
+
       Local Ltac start_good :=
-        apply Compile.rewrite_rules_goodT_by_curried;
-        split; [ reflexivity | ];
-        lazymatch goal with
-        | [ |- forall x p x' p', In (@existT ?A ?P x p, @existT ?A' ?P' x' p') ?ls -> @?Q x x' p p' ]
-          => apply (@forall_In_pair_existT A A' P P' Q ls); cbn [projT1 projT2 fst snd]; cbv [id]
-        end;
-        (exists eq_refl);
-        cbn [eq_rect];
-        cbv [Compile.wf_deep_rewrite_ruleTP_gen Compile.wf_rewrite_rule_data_curried Compile.rew_replacement Compile.rew_should_do_again Compile.rew_with_opt Compile.rew_under_lets Compile.wf_with_unif_rewrite_ruleTP_gen_curried Compile.wf_with_unification_resultT pattern.pattern_of_anypattern pattern.type_of_anypattern Compile.wf_maybe_under_lets_expr Compile.wf_maybe_do_again_expr Compile.wf_with_unification_resultT pattern.type.under_forall_vars_relation Compile.with_unification_resultT' pattern.collect_vars pattern.type.collect_vars pattern.base.collect_vars PositiveSet.empty PositiveSet.elements Compile.under_type_of_list_relation_cps pattern.ident.arg_types pattern.type.subst_default pattern.base.subst_default pattern.base.lookup_default PositiveSet.rev PositiveMap.empty Compile.under_with_unification_resultT_relation_hetero Compile.under_with_unification_resultT'_relation_hetero Compile.maybe_option_eq];
-        cbn [List.map List.fold_right PositiveSet.union PositiveSet.xelements List.rev List.app projT1 projT2 list_rect PositiveSet.add PositiveSet.rev PositiveSet.rev_append PositiveMap.add PositiveMap.find orb];
-        repeat first [ progress intros
-                     | match goal with
-                       | [ |- { pf : ?x = ?x | _ } ] => (exists eq_refl)
-                       end
-                     | progress cbn [eq_rect] in * ].
+        match goal with
+        | [ |- rewrite_rules_goodT ?rew1 ?rew2 ]
+          => let H := fresh in
+             pose proof (@Compile.rewrite_rules_goodT_by_curried _ _ _ _ _ rew1 rew2 eq_refl) as H;
+             let data := lazymatch rew1 with rewrite_rules ?data _ => data end in
+             let h := head data in
+             cbv [h rewrite_rules] in H;
+             let h' := lazymatch type of H with
+                       | context[Compile.rewrite_rules_goodT_curried_cps ?pident_arg_types ?rew1] => head rew1
+                       end in
+             let pident_arg_types
+                 := lazymatch type of H with
+                    | context[Compile.rewrite_rules_goodT_curried_cps ?pident_arg_types ?rew1] => pident_arg_types
+                    end in
+             cbv [h' pident_arg_types Compile.rewrite_rules_goodT_curried_cps] in H;
+             (* make [Qed] not take forever by explicitly recording a cast node *)
+             let H' := fresh in
+             pose proof H as H'; clear H;
+             apply H'; clear H'; intros
+        end.
 
       Local Ltac fin_wf :=
         repeat first [ progress intros
@@ -286,15 +153,16 @@ Module Compilers.
                      | progress intros
                      | progress fin_wf ].
 
+      Local Notation nbe_rewrite_rules := (rewrite_rules nbe_rewriter_data _).
       Lemma nbe_rewrite_rules_good
         : rewrite_rules_goodT nbe_rewrite_rules nbe_rewrite_rules.
       Proof using Type.
         Time start_good.
-        Time all: handle_reified_rewrite_rules; handle_extra_nbe.
+        Time all: abstract (handle_reified_rewrite_rules; handle_extra_nbe).
       Qed.
 
       Local Ltac handle_extra_arith_rules :=
-        repeat first [ progress cbv [rwhenl option_eq SubstVarLike.is_var_fst_snd_pair_opp_cast]
+        repeat first [ progress cbv [option_eq SubstVarLike.is_var_fst_snd_pair_opp_cast] in *
                      | break_innermost_match_step
                      | match goal with
                        | [ Hwf : Compile.wf_value _ ?x _, H : context[SubstVarLike.is_recursively_var_or_ident _ ?x] |- _ ] => erewrite SubstVarLike.wfT_is_recursively_var_or_ident in H by exact Hwf
@@ -302,37 +170,42 @@ Module Compilers.
                      | congruence
                      | progress fin_wf ].
 
+      Local Notation arith_rewrite_rules max_const := (rewrite_rules (arith_rewriter_data max_const) _).
       Lemma arith_rewrite_rules_good max_const
         : rewrite_rules_goodT (arith_rewrite_rules max_const) (arith_rewrite_rules max_const).
       Proof using Type.
         Time start_good.
         Time all: handle_reified_rewrite_rules; handle_extra_arith_rules.
-      Qed.
+      Time Qed.
 
+      Local Notation arith_with_casts_rewrite_rules := (rewrite_rules arith_with_casts_rewriter_data _).
       Lemma arith_with_casts_rewrite_rules_good
         : rewrite_rules_goodT arith_with_casts_rewrite_rules arith_with_casts_rewrite_rules.
       Proof using Type.
         Time start_good.
         Time all: handle_reified_rewrite_rules.
-      Qed.
+      Time Qed.
 
+      Local Notation strip_literal_casts_rewrite_rules := (rewrite_rules strip_literal_casts_rewriter_data _).
       Lemma strip_literal_casts_rewrite_rules_good
         : rewrite_rules_goodT strip_literal_casts_rewrite_rules strip_literal_casts_rewrite_rules.
       Proof using Type.
         Time start_good.
         Time all: handle_reified_rewrite_rules.
-      Qed.
+      Time Qed.
 
+      Local Notation fancy_rewrite_rules invert_low invert_high := (rewrite_rules (fancy_rewriter_data invert_low invert_high) _).
       Lemma fancy_rewrite_rules_good
             (invert_low invert_high : Z -> Z -> option Z)
             (Hlow : forall s v v', invert_low s v = Some v' -> v = Z.land v' (2^(s/2)-1))
             (Hhigh : forall s v v', invert_high s v = Some v' -> v = Z.shiftr v' (s/2))
-        : rewrite_rules_goodT fancy_rewrite_rules fancy_rewrite_rules.
+        : rewrite_rules_goodT (fancy_rewrite_rules invert_low invert_high) (fancy_rewrite_rules invert_low invert_high).
       Proof using Type.
         Time start_good.
         Time all: handle_reified_rewrite_rules.
-      Qed.
+      Time Qed.
 
+      Local Notation fancy_with_casts_rewrite_rules invert_low invert_high value_range flag_range := (rewrite_rules (fancy_with_casts_rewriter_data invert_low invert_high value_range flag_range) _).
       Lemma fancy_with_casts_rewrite_rules_good
             (invert_low invert_high : Z -> Z -> option Z)
             (value_range flag_range : ZRange.zrange)
@@ -342,7 +215,7 @@ Module Compilers.
       Proof using Type.
         Time start_good.
         Time all: handle_reified_rewrite_rules.
-      Qed.
+      Time Qed.
     End good.
   End RewriteRules.
 End Compilers.
