src/RewriterRulesInterpGood.v
@@ -11,33 +11,11 @@ Require Import Crypto.UnderLetsProofs.
 Require Import Crypto.GENERATEDIdentifiersWithoutTypesProofs.
 Require Import Crypto.Rewriter.
 Require Import Crypto.RewriterWf1.
-Require Import Crypto.Util.ZUtil.Tactics.LtbToLt.
-Require Import Crypto.Util.ZUtil.Tactics.DivModToQuotRem.
-Require Import Crypto.Util.ZUtil.Tactics.PullPush.Modulo.
-Require Import Crypto.Util.ZUtil.Hints.
-Require Import Crypto.Util.ZUtil.Hints.Core.
-Require Import Crypto.Util.ZUtil.ZSimplify.Core.
-Require Import Crypto.Util.ZUtil.ZSimplify.
-Require Import Crypto.Util.ZUtil.ZSimplify.Simple.
-Require Import Crypto.Util.ZUtil.Definitions.
-Require Import Crypto.Util.ZUtil.AddGetCarry.
-Require Import Crypto.Util.ZUtil.MulSplit.
-Require Import Crypto.Util.ZUtil.Zselect.
-Require Import Crypto.Util.ZUtil.Div.
-Require Import Crypto.Util.ZUtil.Modulo.
 Require Import Crypto.Util.ZRange.
-Require Import Crypto.Util.ZRange.Operations.
-Require Import Crypto.Util.ZRange.BasicLemmas.
-Require Import Crypto.Util.ZRange.OperationsBounds.
-Require Import Crypto.Util.Tactics.NormalizeCommutativeIdentifier.
+Require Import Crypto.Util.Tactics.UniquePose.
 Require Import Crypto.Util.Tactics.BreakMatch.
 Require Import Crypto.Util.Tactics.SplitInContext.
-Require Import Crypto.Util.Tactics.SpecializeAllWays.
-Require Import Crypto.Util.Tactics.SpecializeBy.
-Require Import Crypto.Util.Tactics.RewriteHyp.
 Require Import Crypto.Util.Tactics.Head.
-Require Import Crypto.Util.Tactics.SetEvars.
-Require Import Crypto.Util.Tactics.SubstEvars.
 Require Import Crypto.Util.Prod.
 Require Import Crypto.Util.Bool.
 Require Import Crypto.Util.ListUtil.
@@ -45,7 +23,6 @@ Require Import Crypto.Util.ListUtil.Forall.
 Require Import Crypto.Util.ListUtil.ForallIn.
 Require Import Crypto.Util.NatUtil.
 Require Import Crypto.Util.Option.
-Require Import Crypto.Util.CPSNotations.
 Require Import Crypto.Util.HProp.
 Require Import Crypto.Util.Decidable.
 Import ListNotations. Local Open Scope list_scope.
@@ -70,81 +47,81 @@ Module Compilers.
       Context {cast_outside_of_range : zrange -> Z -> Z}.
 
       Local Notation ident_interp := (@ident.gen_interp cast_outside_of_range).
-
-      Local Lemma rlist_rect_eq {var A P ivar} Pnil Pcons ls
-        : @rlist_rect var A P ivar Pnil Pcons ls
-          = match invert_expr.reflect_list ls with
-            | Some ls
-              => Some (list_rect
-                         (fun _ => _)
-                         Pnil
-                         (fun x xs rec => rec' <-- rec; Pcons x xs rec')
-                         ls)%under_lets
-            | None => None
-            end.
-      Proof. cbv [rlist_rect Compile.option_bind' Option.bind]; reflexivity. Qed.
-
-      Local Lemma UnderLets_interp_list_rect {A P} Pnil Pcons ls
-        : UnderLets.interp
-            (@ident_interp)
-            (list_rect
-               (fun _ : list A => UnderLets.UnderLets base.type ident _ P)
-               Pnil
-               (fun x xs rec => rec' <-- rec; Pcons x xs rec')
-               ls)%under_lets
-          = list_rect
-              (fun _ => P)
-              (UnderLets.interp (@ident_interp) Pnil)
-              (fun x xs rec => UnderLets.interp (@ident_interp) (Pcons x xs rec))
-              ls.
-      Proof.
-        induction ls as [|x xs IHxs]; cbn [list_rect]; [ reflexivity | ].
-        rewrite UnderLets.interp_splice, IHxs; reflexivity.
-      Qed.
-
-      Local Lemma unfold_is_bounded_by_bool v r
-        : is_bounded_by_bool v r = true -> lower r <= v <= upper r.
-      Proof using Type.
-        cbv [is_bounded_by_bool]; intro; split_andb; Z.ltb_to_lt; split; assumption.
-      Qed.
-
-      Local Lemma unfold_is_tighter_than_bool r1 r2
-        : is_tighter_than_bool r1 r2 = true -> lower r2 <= lower r1 /\ upper r1 <= upper r2.
-      Proof using Type.
-        cbv [is_tighter_than_bool]; intro; split_andb; Z.ltb_to_lt; split; assumption.
-      Qed.
-
       Local Notation rewrite_rules_interp_goodT := (@Compile.rewrite_rules_interp_goodT ident pattern.ident (@pattern.ident.arg_types) (@pattern.ident.to_typed) (@ident_interp)).
 
-      Local Ltac do_cbv0 :=
-        cbv [id
-               Compile.rewrite_rules_interp_goodT_curried
-               Compile.rewrite_rule_data_interp_goodT_curried Compile.under_with_unification_resultT_relation_hetero Compile.under_with_unification_resultT'_relation_hetero Compile.wf_with_unification_resultT Compile.under_type_of_list_relation_cps Compile.under_type_of_list_relation1_cps pattern.pattern_of_anypattern pattern.type_of_anypattern Compile.rew_replacement Compile.rew_should_do_again Compile.rew_with_opt Compile.rew_under_lets Compile.wf_with_unification_resultT Compile.pattern_default_interp pattern.type.under_forall_vars_relation pattern.type.under_forall_vars_relation1 Compile.deep_rewrite_ruleTP_gen Compile.with_unification_resultT' pattern.ident.arg_types pattern.type.lam_forall_vars Compilers.pattern.type.lam_forall_vars_gen Compile.pattern_default_interp' pattern.collect_vars PositiveMap.empty pattern.type.collect_vars PositiveSet.elements PositiveSet.union pattern.base.collect_vars PositiveSet.empty PositiveSet.xelements Compile.lam_type_of_list id pattern.ident.to_typed Compile.under_type_of_list_relation_cps Compile.deep_rewrite_ruleTP_gen_good_relation Compile.normalize_deep_rewrite_rule pattern.type.subst_default PositiveSet.add PositiveSet.rev PositiveSet.rev_append PositiveMap.add Compile.option_bind' Compile.wf_value Compile.value pattern.base.subst_default pattern.base.lookup_default PositiveMap.find Compile.rewrite_ruleTP ident.smart_Literal Compile.value_interp_related
-               Reify.expr_value_to_rewrite_rule_replacement UnderLets.flat_map Compile.reify_expr_beta_iota Compile.reflect_expr_beta_iota Compile.reflect_ident_iota Compile.reify_to_UnderLets UnderLets.of_expr Compile.Base_value];
-        cbn [UnderLets.splice Compile.reflect invert_expr.invert_Literal invert_expr.ident.invert_Literal Compile.splice_under_lets_with_value].
-      Local Ltac do_cbv :=
-        do_cbv0;
-        cbv [List.map List.fold_right List.rev list_rect orb List.app].
-
       Local Ltac start_interp_good :=
-        apply Compile.rewrite_rules_interp_goodT_by_curried;
-        do_cbv;
+        cbv [List.skipn] in *;
         lazymatch goal with
-        | [ |- forall x p, In (@existT ?A ?P x p) ?ls -> @?Q x p ]
-          => let Q' := fresh in
-             pose Q as Q';
-             change (forall x p, In (@existT A P x p) ls -> Q' x p);
-             apply (@forall_In_existT A P Q' ls); subst Q'; cbv [projT1 projT2 id]
+        | [ |- @Compile.rewrite_rules_interp_goodT ?ident ?pident ?pident_arg_types ?pident_to_typed ?ident_interp (rewrite_rules ?data ?var) ]
+          => let H := fresh in
+             pose proof (@Compile.rewrite_rules_interp_goodT_by_curried
+                           _ _ _ pident_to_typed ident_interp (rewrite_rules data var) (rewrite_rules_specs data)) as H;
+             let h := head data in
+             cbv [rewrite_rules dummy_count rewrite_rules_specs h] in * |- ;
+             let h' := lazymatch type of H with context[Compile.rewrite_rules_interp_goodT_curried_cps _ _ _ ?v] => head v end in
+             unfold h' in H at 1;
+             cbv [Compile.rewrite_rules_interp_goodT_curried_cps pident_arg_types pident_to_typed] in H;
+             cbn [snd hd tl projT1 projT2] in H;
+             (* make [Qed] not take forever by explicitly recording a cast node *)
+             let H' := fresh in
+             pose proof H as H'; clear H;
+             apply H'; clear H'
         end;
-        do_cbv0;
-        repeat first [ progress intros
-                     | match goal with
-                       | [ |- { pf : ?x = ?x | _ } ] => (exists eq_refl)
-                       | [ |- True /\ _ ] => split; [ exact I | ]
-                       | [ |- _ /\ _ ] => split; [ intros; exact I | ]
-                       end
-                     | progress cbn [eq_rect] in * ];
-        cbn [fst snd base.interp base.base_interp type.interp projT1 projT2 UnderLets.interp expr.interp type.related ident.gen_interp UnderLets.interp_related UnderLets.interp_related_gen] in *.
+        [ try assumption;
+          cbn [PrimitiveHList.hlist snd];
+          repeat lazymatch goal with
+                 | [ |- PrimitiveProd.Primitive.prod _ _ ] => constructor
+                 | [ |- forall A x, x = x ] => reflexivity
+                 end;
+          try assumption
+        | try match goal with
+              | [ H : PrimitiveHList.hlist _ _ |- _ ] => clear H
+              end;
+          let H := fresh in
+          intro H; hnf in H;
+          repeat first [ progress intros
+                       | match goal with
+                         | [ |- { pf : ?x = ?x | _ } ] => (exists eq_refl)
+                         | [ |- True /\ _ ] => split; [ exact I | ]
+                         | [ |- _ /\ _ ] => split; [ intros; exact I | ]
+                         | [ |- match (if ?b then _ else _) with Some _ => _ | None => _ end ]
+                           => destruct b eqn:?
+                         | [ |- True ] => exact I
+                         end
+                       | progress eta_expand
+                       | progress cbn [eq_rect] in * ];
+          cbn [fst snd base.interp base.base_interp type.interp projT1 projT2 UnderLets.interp expr.interp type.related ident.gen_interp] in *;
+          cbn [fst snd] in *;
+          eta_expand;
+          split_andb;
+          repeat match goal with
+                 | [ H : ?b = true |- _ ] => unique pose proof (@Reflect.reflect_bool _ b _ H)
+                 | [ H : negb _ = false |- _ ] => rewrite Bool.negb_false_iff in H
+                 | [ H : _ = false |- _ ] => rewrite <- Bool.negb_true_iff in H
+                 end;
+          subst; cbv [ident.gets_inlined ident.literal] in *;
+          lazymatch goal with
+          | [ |- ?R ?v ]
+            => let v' := open_constr:(_) in
+               replace v with v';
+               [ | symmetry;
+                   unshelve eapply H; shelve_unifiable;
+                   try eassumption;
+                   try (repeat apply conj; assumption);
+                   try match goal with
+                       | [ |- ?A = ?B ] => first [ is_evar A | is_evar B ]; reflexivity
+                       | [ |- ?T ] => is_evar T; exact I
+                       | [ |- ?P ] (* TODO: Maybe we shouldn't simplify boolean expressions in rewriter reification, since we end up just having to undo it here in a kludgy way....... *)
+                         => apply (proj2 (@Bool.reflect_iff P _ _));
+                            progress rewrite ?Bool.eqb_true_l, ?Bool.eqb_true_r, ?Bool.eqb_false_l, ?Bool.eqb_false_r;
+                            let b := lazymatch goal with |- ?b = true => b end in
+                            apply (proj1 (@Bool.reflect_iff _ b _));
+                            tauto
+                       end ];
+               clear H
+          end;
+          fold (@base.interp) in *
+                                 .. ].
 
       Ltac recurse_interp_related_step :=
         let do_replace v :=
@@ -192,767 +169,230 @@ Module Compilers.
         end.
 
       (* TODO: MOVE ME? *)
-      Local Ltac recursive_match_to_list_case term :=
+      Local Ltac recursive_match_to_case term :=
+        let contains_match x
+            := lazymatch x with
+               | context[match _ with nil => _ | _ => _ end] => true
+               | context[match _ with pair a b => _ end] => true
+               | context[match _ with true => _ | false => _ end] => true
+               | _ => false
+               end in
         lazymatch term with
         | context G[match ?ls with nil => ?N | cons x xs => @?C x xs end]
           => let T := type of N in
              let term := context G[list_case (fun _ => T) N C ls] in
-             recursive_match_to_list_case term
-        | context[match _ with nil => _ | _ => _ end]
-          => let G_f
-                 := match term with
-                    | context G[fun x : ?T => @?f x]
-                      => lazymatch f with
-                         | context[match _ with nil => _ | _ => _ end]
-                           => let f' := fresh in
-                              let T' := type of f in
-                              constr:(((fun f' : T' => ltac:(let G' := context G[f'] in exact G')),
-                                       f))
-                         end
-                    end in
-             lazymatch G_f with
-             | ((fun f' => ?G), (fun x : ?T => ?f))
-               => let x' := fresh in
-                  let rep := constr:(fun x' : T
-                                     => ltac:(let f := constr:(match x' with x => f end) in
-                                              let f := recursive_match_to_list_case f in
-                                              exact f)) in
-                  let term := constr:(match rep with f' => G end) in
-                  recursive_match_to_list_case term
-             end
-        | _ => term
+             recursive_match_to_case term
+        | context G[match ?v with pair a b => @?P a b end]
+          => let T := lazymatch type of P with forall a b, @?T a b => T end in
+             let term := context G[prod_rect (fun ab => T (fst ab) (snd ab)) P v] in
+             recursive_match_to_case term
+        | context G[match ?b with true => ?t | false => ?f end]
+          => let T := type of t in
+             let term := context G[bool_rect (fun _ => T) t f b] in
+             recursive_match_to_case term
+        | _ => let has_match := contains_match term in
+               match has_match with
+               | true
+                 => let G_f
+                        := match term with
+                           | context G[fun x : ?T => @?f x]
+                             => let has_match := contains_match f in
+                                lazymatch has_match with
+                                | true
+                                  => let f' := fresh in
+                                     let T' := type of f in
+                                     constr:(((fun f' : T' => ltac:(let G' := context G[f'] in exact G')),
+                                              f))
+                                end
+                           end in
+                    lazymatch G_f with
+                    | ((fun f' => ?G), (fun x : ?T => ?f))
+                      => let x' := fresh in
+                         let rep := constr:(fun x' : T
+                                            => ltac:(let f := constr:(match x' with x => f end) in
+                                                     let f := recursive_match_to_case f in
+                                                     exact f)) in
+                         let term := constr:(match rep with f' => G end) in
+                         recursive_match_to_case term
+                    end
+               | false
+                 => term
+               end
         end.
-      Local Ltac recursive_match_to_list_case_in_goal :=
+      Local Ltac recursive_match_to_case_in_goal :=
         let G := match goal with |- ?G => G end in
-        let G := recursive_match_to_list_case G in
+        let G := recursive_match_to_case G in
         change G.
 
-      Local Ltac interp_good_t_step_related :=
-        first [ lazymatch goal with
-                | [ |- ?x = ?x ] => reflexivity
-                | [ |- True ] => exact I
-                | [ H : ?x = true, H' : ?x = false |- _ ] => exfalso; clear -H H'; congruence
-                | [ |- ?G ] => has_evar G; reflexivity
-                | [ |- context[expr.interp_related_gen _ _ _ _] ] => reflexivity
-                | [ |- context[_ == _] ] => reflexivity
-                (*| [ |- context[(fst ?x, snd ?x)] ] => progress eta_expand
-                | [ |- context[match ?x with pair a b => _ end] ] => progress eta_expand*)
-                end
-              | match goal with
-                | [ |- UnderLets.interp_related ?ii ?R (UnderLets.Base (#ident.list_rect @ _ @ _ @ _)%expr) (@list_rect ?A (fun _ => ?P) ?N ?C ?ls) ]
-                  => progress change (@list_rect A (fun _ => P) N C ls) with (@ident.Thunked.list_rect A P (fun _ => N) C ls)
-                | [ |- expr.interp_related_gen ?ii ?R (#ident.list_rect @ _ @ _ @ _)%expr (@list_rect ?A (fun _ => ?P) ?N ?C ?ls) ]
-                  => progress change (@list_rect A (fun _ => P) N C ls) with (@ident.Thunked.list_rect A P (fun _ => N) C ls)
-                | [ |- expr.interp_related_gen ?ii ?R (#ident.list_case @ _ @ _ @ _)%expr (@list_case ?A (fun _ => ?P) ?N ?C ?ls) ]
-                  => progress change (@list_case A (fun _ => P) N C ls) with (@ident.Thunked.list_case A P (fun _ => N) C ls)
-                | [ |- UnderLets.interp_related _ _ (list_rect _ _ _ _) (List.app ?ls1 ?ls2) ]
-                  => rewrite (eq_app_list_rect ls1 ls2)
-                | [ |- UnderLets.interp_related _ _ (list_rect _ _ _ _) (@flat_map ?A ?B ?f ?ls) ]
-                  => rewrite (@eq_flat_map_list_rect A B f ls)
-                | [ |- UnderLets.interp_related _ _ (list_rect _ _ _ _) (@partition ?A ?f ?ls) ]
-                  => rewrite (@eq_partition_list_rect A f ls)
-                | [ |- UnderLets.interp_related _ _ (list_rect _ _ _ _) (@List.map ?A ?B ?f ?ls) ]
-                  => rewrite (@eq_map_list_rect A B f ls)
-                | [ |- UnderLets.interp_related _ _ (list_rect _ _ _ _ _) (@List.combine ?A ?B ?xs ?ys) ]
-                  => rewrite (@eq_combine_list_rect A B xs ys)
-                | [ |- UnderLets.interp_related _ _ (nat_rect _ _ _ _) (List.repeat ?x ?n) ]
-                  => rewrite (eq_repeat_nat_rect x n)
-                | [ |- ?R (nat_rect _ _ _ _ _) (@List.firstn ?A ?n ?ls) ]
-                  => rewrite (@eq_firstn_nat_rect A n ls)
-                | [ |- ?R (nat_rect _ _ _ _ _) (@List.skipn ?A ?n ?ls) ]
-                  => rewrite (@eq_skipn_nat_rect A n ls)
-                | [ |- ?R (list_rect _ _ _ _) (@List.rev ?A ?xs) ]
-                  => rewrite (@eq_rev_list_rect A xs)
-                | [ |- ?R (list_rect _ _ _ _) (@List.length ?A ?xs) ]
-                  => rewrite (@eq_length_list_rect A xs)
-                | [ |- ?R (list_rect _ _ _ _) (@List.flat_map ?A ?B ?f ?xs) ]
-                  => rewrite (@eq_flat_map_list_rect A B f xs)
-                | [ |- ?R (list_rect _ _ _ _) (@List.partition ?A ?f ?xs) ]
-                  => rewrite (@eq_partition_list_rect A f xs)
-                | [ |- ?R (nat_rect _ _ _ _ _) (@update_nth ?A ?n ?f ?xs) ]
-                  => rewrite (@eq_update_nth_nat_rect A n f xs)
-
-                | [ |- UnderLets.interp_related _ _ (UnderLets.Base (#ident.list_rect @ _ @ _ @ _)%expr) (List.app ?ls1 ?ls2) ]
-                  => rewrite (eq_app_list_rect ls1 ls2)
-                | [ |- UnderLets.interp_related _ _ (UnderLets.Base (#ident.list_rect @ _ @ _ @ _)%expr) (List.app ?ls1 ?ls2) ]
-                  => rewrite (eq_app_list_rect ls1 ls2)
-                | [ |- UnderLets.interp_related _ _ (UnderLets.Base (#ident.list_rect @ _ @ _ @ _)%expr) (@flat_map ?A ?B ?f ?ls) ]
-                  => rewrite (@eq_flat_map_list_rect A B f ls)
-                | [ |- UnderLets.interp_related _ _ (UnderLets.Base (#ident.list_rect @ _ @ _ @ _)%expr) (@partition ?A ?f ?ls) ]
-                  => rewrite (@eq_partition_list_rect A f ls)
-                | [ |- UnderLets.interp_related _ _ (UnderLets.Base (#ident.list_rect @ _ @ _ @ _)%expr) (@List.map ?A ?B ?f ?ls) ]
-                  => rewrite (@eq_map_list_rect A B f ls)
-                | [ |- UnderLets.interp_related _ _ (UnderLets.Base (#ident.list_rect_arrow @ _ @ _ @ _ @ _)%expr) (@List.combine ?A ?B ?xs ?ys) ]
-                  => rewrite (@eq_combine_list_rect A B xs ys)
-                | [ |- UnderLets.interp_related _ _ _ (@fold_right ?A ?B ?f ?v ?ls) ]
-                  => rewrite (@eq_fold_right_list_rect A B f v ls)
-                | [ |- ?R (#ident.nat_rect_arrow @ _ @ _ @ _ @ _)%expr (@List.firstn ?A ?n ?ls) ]
-                  => rewrite (@eq_firstn_nat_rect A n ls)
-                | [ |- ?R (#ident.nat_rect_arrow @ _ @ _ @ _ @ _)%expr (@List.skipn ?A ?n ?ls) ]
-                  => rewrite (@eq_skipn_nat_rect A n ls)
-                | [ |- ?R (#ident.list_rect @ _ @ _ @ _)%expr (@List.rev ?A ?xs) ]
-                  => rewrite (@eq_rev_list_rect A xs)
-                | [ |- ?R (#ident.list_rect @ _ @ _ @ _)%expr (@List.length ?A ?xs) ]
-                  => rewrite (@eq_length_list_rect A xs)
-                | [ |- ?R (#ident.list_rect @ _ @ _ @ _)%expr (@List.flat_map ?A ?B ?f ?xs) ]
-                  => rewrite (@eq_flat_map_list_rect A B f xs)
-                | [ |- ?R (#ident.list_rect @ _ @ _ @ _)%expr (@List.partition ?A ?f ?xs) ]
-                  => rewrite (@eq_partition_list_rect A f xs)
-                | [ |- ?R (#ident.nat_rect_arrow @ _ @ _ @ _ @ _)%expr (@update_nth ?A ?n ?f ?xs) ]
-                  => rewrite (@eq_update_nth_nat_rect A n f xs)
-                | [ |- ?R (#ident.list_rect_arrow @ _ @ _ @ _ @ _)%expr (@List.combine ?A ?B ?xs ?ys) ]
-                  => rewrite (@eq_combine_list_rect A B xs ys)
-
-
-                | [ |- expr.interp_related_gen _ _ (#ident.list_rect @ _ @ _ @ _)%expr (ident.Thunked.list_rect _ _ _ _) ]
-                  => recurse_interp_related_step; [ recurse_interp_related_step | reflexivity ];
-                     [ recurse_interp_related_step; [ recurse_interp_related_step | reflexivity ];
-                       [ recurse_interp_related_step; [ recurse_interp_related_step | reflexivity ];
-                         [ recurse_interp_related_step; [ recurse_interp_related_step | reflexivity ]
-                         | ]
-                       | ]
-                     | ]
-                | [ |- expr.interp_related_gen _ _ (#ident.list_rect_arrow @ _ @ _ @ _ @ _)%expr (list_rect _ _ _ _ _) ]
-                  => recurse_interp_related_step; [ recurse_interp_related_step | reflexivity ];
-                     [ recurse_interp_related_step; [ recurse_interp_related_step | reflexivity ];
-                       [ recurse_interp_related_step; [ recurse_interp_related_step | reflexivity ];
-                         [ recurse_interp_related_step; [ recurse_interp_related_step | reflexivity ];
-                           [ recurse_interp_related_step; [ recurse_interp_related_step | reflexivity ]
-                           | ]
-                         | ]
-                       | ]
-                     | ]
-                | [ |- expr.interp_related_gen _ _ (#ident.nat_rect @ _ @ _ @ _)%expr (ident.Thunked.nat_rect _ _ _ _) ]
-                  => recurse_interp_related_step; [ recurse_interp_related_step | reflexivity ];
-                     [ recurse_interp_related_step; [ recurse_interp_related_step | reflexivity ];
-                       [ recurse_interp_related_step; [ recurse_interp_related_step | reflexivity ];
-                         [ recurse_interp_related_step; [ recurse_interp_related_step | reflexivity ]
-                         | ]
-                       | ]
-                     | ]
-                | [ |- expr.interp_related_gen _ _ (#ident.nat_rect_arrow @ _ @ _ @ _ @ _)%expr (nat_rect _ _ _ _ _) ]
-                  => recurse_interp_related_step; [ recurse_interp_related_step | reflexivity ];
-                     [ recurse_interp_related_step; [ recurse_interp_related_step | reflexivity ];
-                       [ recurse_interp_related_step; [ recurse_interp_related_step | reflexivity ];
-                         [ recurse_interp_related_step; [ recurse_interp_related_step | reflexivity ];
-                           [ recurse_interp_related_step; [ recurse_interp_related_step | reflexivity ]
-                           | ]
-                         | ]
-                       | ]
-                     | ]
-                | [ |- expr.interp_related_gen _ _ (#ident.list_case @ _ @ _ @ _)%expr (ident.Thunked.list_case _ _ _ _) ]
-                  => recurse_interp_related_step; [ recurse_interp_related_step | reflexivity ];
-                     [ recurse_interp_related_step; [ recurse_interp_related_step | reflexivity ];
-                       [ recurse_interp_related_step; [ recurse_interp_related_step | reflexivity ];
-                         [ recurse_interp_related_step; [ recurse_interp_related_step | reflexivity ]
-                         | ]
-                       | ]
-                     | ]
-                | [ |- context[match _ with nil => _ | _ => _ end] ] => progress recursive_match_to_list_case_in_goal
-                end
-              | progress cbn [expr.interp ident.gen_interp fst snd Compile.reify Compile.reflect Compile.wf_value' Compile.value' Option.bind UnderLets.interp list_case type.interp base.interp base.base_interp ident.to_fancy invert_Some ident.fancy.interp ident.fancy.interp_with_wordmax Compile.reify_expr bool_rect UnderLets.interp_related UnderLets.interp_related_gen type.related] in *
-              | progress cbv [Compile.option_bind' respectful expr.interp_related] in *
-              | progress fold (@type.interp _ base.interp)
-              | progress fold (@base.interp)
-              | progress change S with Nat.succ
-              | match goal with
-                | [ |- context[List.map _ (Lists.List.repeat _ _)] ] => rewrite map_repeat
-                | [ |- context[List.map _ (List.map _ _)] ] => rewrite map_map
-                | [ |- context[List.map (fun x => x) _] ] => rewrite map_id
-                | [ |- context[List.map _ (List.rev _)] ] => rewrite map_rev
-                | [ |- context[List.map _ (firstn _ _)] ] => rewrite <- firstn_map
-                | [ |- context[List.map _ (skipn _ _)] ] => rewrite <- skipn_map
-                | [ |- context[List.length (List.map _ _)] ] => rewrite map_length
-                | [ |- context[List.combine (List.map _ _) _] ] => rewrite combine_map_l
-                | [ |- context[List.combine _ (List.map _ _)] ] => rewrite combine_map_r
-                | [ |- context[expr.interp _ (reify_list _)] ] => rewrite expr.interp_reify_list
-                | [ |- context[expr.interp _ (UnderLets.to_expr ?e)] ] => rewrite UnderLets.interp_to_expr
-                | [ |- context[UnderLets.interp _ (UnderLets.splice_list _ _)] ] => rewrite UnderLets.interp_splice_list
-                | [ |- context[rlist_rect] ] => rewrite rlist_rect_eq
-                | [ |- context[UnderLets.interp _ (list_rect _ _ _ _)] ] => rewrite UnderLets_interp_list_rect
-                | [ |- context[UnderLets.interp _ (UnderLets.splice _ _)] ] => rewrite UnderLets.interp_splice
-                | [ |- context[list_rect _ _ _ (List.map _ _)] ] => rewrite list_rect_map
-                | [ |- context[expr.interp_related_gen _ _ (reify_list _)] ]
-                  => rewrite expr.reify_list_interp_related_gen_iff
-                | [ H : context[expr.interp_related_gen _ _ (reify_list _)] |- _ ]
-                  => rewrite expr.reify_list_interp_related_gen_iff in H
-                | [ |- expr.interp_related_gen ?ident_interp _ (UnderLets.to_expr ?x) ?y ]
-                  => change (expr.interp_related ident_interp (UnderLets.to_expr x) y);
-                     rewrite <- UnderLets.to_expr_interp_related_iff
-                | [ |- context[Forall2 _ (List.map _ _) _] ] => rewrite Forall2_map_l_iff
-                | [ |- context[Forall2 _ _ (List.map _ _)] ] => rewrite Forall2_map_r_iff
-                | [ |- context[Forall2 _ (List.repeat _ _) (List.repeat _ _)] ] => rewrite Forall2_repeat_iff
-                | [ |- context[Forall2 _ (List.rev _) (List.rev _)] ] => rewrite Forall2_rev_iff
-                | [ |- context[Forall2 _ ?x ?x] ] => rewrite Forall2_Forall; cbv [Proper]
-                | [ |- context[Forall _ (seq _ _)] ] => rewrite Forall_seq
-                | [ H : Forall2 ?R ?l1 ?l2 |- Forall2 ?R (List.firstn ?n ?l1) (List.firstn ?n ?l2) ]
-                  => apply Forall2_firstn, H
-                | [ H : Forall2 ?R ?l1 ?l2 |- Forall2 ?R (List.skipn ?n ?l1) (List.skipn ?n ?l2) ]
-                  => apply Forall2_skipn, H
-                | [ |- Forall2 ?R (List.combine _ _) (List.combine _ _) ]
-                  => eapply Forall2_combine; [ | eassumption | eassumption ]
-                | [ H : List.Forall2 _ ?l1 ?l2, H' : ?R ?v1 ?v2 |- ?R (nth_default ?v1 ?l1 ?x) (nth_default ?v2 ?l2 ?x) ]
-                  => apply Forall2_forall_iff''; split; assumption
-                | [ H : List.Forall2 _ ?x ?y |- List.length ?x = List.length ?y ]
-                  => eapply eq_length_Forall2, H
-                | [ |- exists fv xv, _ /\ _ /\ fv xv = ?f ?x ]
-                  => exists f, x; repeat apply conj; [ solve [ repeat interp_good_t_step_related ] | | reflexivity ]
-                | [ |- _ /\ ?x = ?x ] => split; [ | reflexivity ]
-                | [ |- UnderLets.interp_related
-                         ?ident_interp ?R
-                         (list_rect
-                            (fun _ : list (expr ?A) => UnderLets.UnderLets _ _ _ ?B)
-                            ?Pnil
-                            ?Pcons
-                            ?ls)
-                         (list_rect
-                            (fun _ : list _ => ?B')
-                            ?Pnil'
-                            ?Pcons'
-                            ?ls') ]
-                  => apply (@UnderLets.list_rect_interp_related _ _ _ ident_interp A B Pnil Pcons ls B' Pnil' Pcons' ls' R)
-                | [ |- UnderLets.interp_related
-                         ?ident_interp ?R
-                         (list_rect
-                            (fun _ : list (expr ?A) => ?B -> UnderLets.UnderLets _ _ _ ?C)
-                            ?Pnil
-                            ?Pcons
-                            ?ls
-                            ?x)
-                         (list_rect
-                            (fun _ : list _ => ?B' -> ?C')
-                            ?Pnil'
-                            ?Pcons'
-                            ?ls'
-                            ?x') ]
-                  => apply (@UnderLets.list_rect_arrow_interp_related _ _ _ ident_interp A B C Pnil Pcons ls x B' C' Pnil' Pcons' ls' x' R (expr.interp_related ident_interp))
-                | [ |- UnderLets.interp_related _ _ (nat_rect _ _ _ _) (nat_rect _ _ _ _) ]
-                  => apply UnderLets.nat_rect_interp_related
-                | [ |- UnderLets.interp_related _ _ (nat_rect _ _ _ _ _) (nat_rect _ _ _ _ _) ]
-                  => eapply UnderLets.nat_rect_arrow_interp_related; [ .. | eassumption ]
-                | [ |- UnderLets.interp_related _ _ (UnderLets.splice _ _) _ ]
-                  => rewrite UnderLets.splice_interp_related_iff
-                | [ |- UnderLets.interp_related ?ident_interp _ (UnderLets.splice_list _ _) _ ]
-                  => apply UnderLets.splice_list_interp_related_of_ex with (RA:=expr.interp_related ident_interp); exists (fun x => x); eexists; repeat apply conj; [ | | reflexivity ]
-                | [ H : UnderLets.interp_related _ _ ?e ?v1 |- UnderLets.interp_related _ _ ?e ?f ]
-                  => let f := match (eval pattern v1 in f) with ?f _ => f end in
-                     eapply (@UnderLets.interp_related_Proper_impl_same_UnderLets _ _ _ _ _ _ _ _ _ e v1 f); [ | exact H ]; cbv beta
-                | [ H : forall x y, ?R x y -> UnderLets.interp_related _ _ (?e x) (?v1 y) |- UnderLets.interp_related _ _ (?e ?xv) ?f ]
-                  => lazymatch f with
-                     | context[v1 ?yv]
-                       => let f := match (eval pattern (v1 yv) in f) with ?f _ => f end in
-                          eapply (@UnderLets.interp_related_Proper_impl_same_UnderLets _ _ _ _ _ _ _ _ _ (e xv) (v1 yv) f); [ | eapply H; assumption ]
-                     end
-                | [ |- expr.interp_related_gen
-                         _ _
-                         (#(ident.prod_rect) @ ?f @ ?e)%expr
-                         match ?e' with pair a b => @?f' a b end ]
-                  => let fh := fresh in
-                     let eh := fresh in
-                     set (fh := f); set (eh := e); cbn [expr.interp_related_gen]; subst fh eh;
-                     exists (fun ev => match ev with pair a b => f' a b end), e';
-                     repeat apply conj;
-                     [ | assumption | reflexivity ];
-                     exists (fun fv ev => match ev with pair a b => fv a b end), f';
-                     repeat apply conj;
-                     [ cbn [type.interp type.related ident_interp]; cbv [respectful]; intros; subst; eta_expand; auto | | reflexivity ]
-                | [ |- expr.interp_related_gen
-                         _ _
-                         (#(ident.bool_rect) @ ?t @ ?f @ ?b)%expr
-                         (bool_rect ?P ?t' ?f' ?b') ]
-                  => let th := fresh in
-                     let fh := fresh in
-                     let bh := fresh in
-                     set (th := t); set (fh := f); set (bh := b); cbn [expr.interp_related_gen]; subst th fh bh;
-                     unshelve
-                       ((exists (bool_rect P t' f'), b'); repeat apply conj;
-                        [ | shelve | reflexivity ];
-                        (exists (fun fv => bool_rect P t' (fv tt)), (fun _ => f')); repeat apply conj;
-                        [ | shelve | reflexivity ];
-                        (exists (fun tv fv => bool_rect P (tv tt) (fv tt)), (fun _ => t')); repeat apply conj;
-                        [ | shelve | reflexivity ])
-                | [ |- @expr.interp_related_gen _ _ _ _ _ _ (type.base ?t) _ _ ]
-                  => lazymatch t with
-                     | base.type.type_base base.type.Z => idtac
-                     | base.type.prod (base.type.type_base base.type.Z) (base.type.type_base base.type.Z) => idtac
-                     end;
-                     progress repeat recurse_interp_related_step
-                | [ |- exists (fv : ?T1 -> ?T2) (ev : ?T1),
-                      _ /\ _ /\ fv ev = ?x ]
-                  => lazymatch T1 with Z => idtac | (Z * Z)%type => idtac end;
-                     lazymatch T2 with Z => idtac | (Z * Z)%type => idtac end;
-                     progress repeat recurse_interp_related_step
-                | [ |- expr.interp_related_gen _ _ (expr.Abs ?f) _ ]
-                  => let fh := fresh in set (fh := f); cbn [expr.interp_related_gen]; subst fh
-                | [ H : expr.interp_related_gen _ _ ?x ?x' |- expr.interp_related_gen _ _ (?f @ ?x) (?f' ?x') ]
-                  => let fh := fresh in
-                     let xh := fresh in
-                     set (fh := f); set (xh := x); cbn [expr.interp_related_gen]; subst fh xh;
-                     exists f', x'; repeat apply conj;
-                     [ | exact H | reflexivity ]
-                | [ |- List.Forall2 _ (update_nth _ _ _) (update_nth _ _ _) ] => apply Forall2_update_nth
-                | [ H : zrange * zrange |- _ ] => destruct H
-                end
+      Local Ltac preprocess_step :=
+        first [ progress cbv [expr.interp_related respectful ident.literal ident.eagerly] in *
+              | progress cbn [fst snd base.interp base.base_interp Compile.value'] in *
               | progress intros
               | progress subst
-              | assumption
-              | progress inversion_option
-              | progress destruct_head'_and
-              | progress destruct_head'_unit
-              | progress split_andb
               | match goal with
-                | [ |- Lists.List.repeat _ _ = Lists.List.repeat _ _ ] => apply f_equal2
-                | [ |- firstn _ _ = firstn _ _ ] => apply f_equal2
-                | [ |- skipn _ _ = skipn _ _ ] => apply f_equal2
-                | [ |- rev _ = rev _ ] => apply f_equal
-                | [ |- List.app ?l1 ?l2 = List.app ?l1' ?l2 ] => apply f_equal2
-                | [ |- List.app ?l1 ?l2 = List.app ?l1 ?l2' ] => apply f_equal2
-                | [ |- cons _ _ = cons _ _ ] => apply f_equal2
-                | [ |- list_rect _ ?Pnil ?Pcons ?ls = list_rect _ ?Pnil ?Pcons' ?ls ]
-                  => apply list_rect_Proper; [ reflexivity | repeat intro | reflexivity ]
-                | [ |- bool_rect _ ?x ?y ?b = bool_rect _ ?x ?y ?b' ]
-                  => apply f_equal3; [ reflexivity | reflexivity | solve [ repeat interp_good_t_step_related ] ]
-                | [ H : expr.wf _ ?v1 ?v2 |- expr.interp _ ?v1 = expr.interp _ ?v2 ]
-                  => apply (expr.wf_interp_Proper _ _ _ H ltac:(assumption))
-                | [ |- ?R (?f (?g (if ?b then ?x else ?y))) (bool_rect ?A ?B ?C ?D) ]
-                  => rewrite <- (@Bool.pull_bool_if _ _ g b), <- (@Bool.pull_bool_if _ _ f b);
-                     change (R (bool_rect _ (f (g x)) (f (g y)) b) (bool_rect A B C D))
-                | [ |- context[invert_expr.reflect_list ?ls] ]
-                  => destruct (invert_expr.reflect_list ls) eqn:?; expr.invert_subst
-                | [ |- ?f (nth_default _ _ _) = _ ]
-                  => rewrite <- (@map_nth_default_always _ _ f)
-                | [ |- map ?f ?ls = map ?g ?ls ] => apply map_ext_in
-                | [ |- List.map _ (update_nth _ _ _) = update_nth _ _ _ ] => apply map_update_nth_ext
-                | [ H : ?x = ?x -> _ |- _ ] => specialize (H eq_refl)
-                | [ H : forall v : unit, _ |- _ ] => specialize (H tt)
-                | [ H : _ = expr.interp ?ii ?v |- _ ] => is_var v; generalize dependent (expr.interp ii v); clear v
-                | [ |- bool_rect _ _ _ ?b = bool_rect _ _ _ ?b ]
-                  => is_var b; destruct b; cbv [bool_rect]
-                | [ H : (forall x y, _ -> expr.interp _ (UnderLets.interp _ (?f1 x)) = expr.interp _ (UnderLets.interp _ (?f2 y)))
-                    |- expr.interp _ (UnderLets.interp _ (?f1 ?x1)) = expr.interp _ (UnderLets.interp _ (?f2 ?x2)) ]
-                  => apply H
-                | [ H : (forall x y, _ -> forall x' y', _ -> expr.interp _ (UnderLets.interp _ (?f1 x x')) = expr.interp _ (UnderLets.interp _ (?f2 y y')))
-                    |- expr.interp _ (UnderLets.interp _ (?f1 ?x1 ?y1)) = expr.interp _ (UnderLets.interp _ (?f2 ?x2 ?y2)) ]
-                  => apply H
-                | [ |- context G[rwhen ?v ?b] ]
-                  => let c := constr:(rwhen v b) in
-                     let c := (eval cbv [rwhen] in c) in
-                     let G' := context G[c] in
-                     change G';
-                     destruct b eqn:?
-                | [ |- context G[rwhenl ?v ?b] ]
-                  => let c := constr:(rwhenl v b) in
-                     let c := (eval cbv [rwhenl] in c) in
-                     let G' := context G[c] in
-                     change G';
-                     destruct b eqn:?
-                | [ H : negb ?b = true |- _ ] => rewrite (@Bool.negb_true_iff b) in H
-                | [ |- context[expr.interp ?ii ?v] ]
-                  => is_var v; generalize dependent (expr.interp ii v); clear v; intro v
-                | [ |- context[Z.mul_split ?a ?b ?c] ]
-                  => rewrite (surjective_pairing (Z.mul_split a b c)), Z.mul_split_div, Z.mul_split_mod
-                | [ |- context[Z.zselect] ] => rewrite Z.zselect_correct
-                | [ |- context[Z.sub_get_borrow_full ?a ?b ?c] ]
-                  => rewrite (surjective_pairing (Z.sub_get_borrow_full a b c)), Z.sub_get_borrow_full_div, Z.sub_get_borrow_full_mod
-                | [ |- context[Z.sub_with_get_borrow_full ?a ?b ?c ?d] ]
-                  => rewrite (surjective_pairing (Z.sub_with_get_borrow_full a b c d)), Z.sub_with_get_borrow_full_div, Z.sub_with_get_borrow_full_mod
-                | [ |- context[Z.add_get_carry_full ?a ?b ?c] ]
-                  => rewrite (surjective_pairing (Z.add_get_carry_full a b c)), Z.add_get_carry_full_div, Z.add_get_carry_full_mod
-                | [ |- context[Z.add_with_get_carry_full ?a ?b ?c ?d] ]
-                  => rewrite (surjective_pairing (Z.add_with_get_carry_full a b c d)), Z.add_with_get_carry_full_div, Z.add_with_get_carry_full_mod
-                | [ |- pair _ _ = pair _ _ ] => apply f_equal2
-                | [ |- ?a mod ?b = ?a' mod ?b ] => apply f_equal2; lia
-                | [ |- ?a / ?b = ?a' / ?b ] => apply f_equal2; lia
-                | [ |- Z.opp _ = Z.opp _ ] => apply f_equal
-                end
-              | match goal with
-                | [ |- context[?f (list_rect _ _ _ _)] ]
-                  => match f with
-                     | expr.interp _ => idtac
-                     | Compile.reify_expr => idtac
-                     end;
-                     erewrite (@push_f_list_rect _ _ f)
-                       by (intros;
-                           repeat first [ progress cbn [expr.interp ident.gen_interp UnderLets.interp Compile.reify_expr]
-                                        | rewrite UnderLets.interp_splice ];
-                           match goal with
-                           | [ |- ?LHS = ?Pcons' ?x ?xs ?rec ]
-                             => let LHS' := match (eval pattern x, xs, rec in LHS) with ?f _ _ _ => f end in
-                                unify Pcons' LHS'; reflexivity
-                           end)
-                | [ |- context[?f (nat_rect _ _ _ _)] ]
-                  => match f with
-                     | expr.interp _ => idtac
-                     | UnderLets.interp _ => idtac
-                     | Compile.reify_expr => idtac
-                     end;
-                     erewrite (@push_f_nat_rect _ _ f)
-                       by (intros;
-                           repeat first [ progress cbn [expr.interp ident.gen_interp UnderLets.interp Compile.reify_expr]
-                                        | rewrite UnderLets.interp_splice ];
-                           match goal with
-                           | [ |- ?LHS = ?PS' ?x ?rec ]
-                             => let LHS' := match (eval pattern x, rec in LHS) with ?f _ _ => f end in
-                                unify PS' LHS'; reflexivity
-                           end)
-                | [ |- ?f (list_rect _ _ _ _) = list_rect _ _ _ _ ]
-                  => match f with
-                     | expr.interp _ => idtac
-                     | Compile.reify_expr => idtac
-                     end;
-                     erewrite (@push_f_list_rect _ _ f);
-                     [ apply list_rect_Proper; repeat intro; try reflexivity | ]
-                | [ |- ?f (nat_rect _ _ _ _) = nat_rect _ _ _ _ ]
-                  => match f with
-                     | expr.interp _ => idtac
-                     | UnderLets.interp _ => idtac
-                     | Compile.reify_expr => idtac
-                     end;
-                     erewrite (@push_f_nat_rect _ _ f);
-                     [ apply nat_rect_Proper_nondep; repeat intro; try reflexivity | ]
-                end
-              | break_innermost_match_step
-              | break_innermost_match_hyps_step
-              | progress destruct_head'_or
-              | progress cbn [expr.interp_related_gen] in *
-              | match goal with
-                | [ H : context[expr.interp _ (UnderLets.interp _ (?f _ _ _))]
-                    |- expr.interp _ (UnderLets.interp _ (?f _ _ _)) = _ ]
-                  => apply H
-                | [ H : forall x1 x2, ?R1 x1 x2 -> ?R2 (?f1 x1) (?f2 x2) |- ?R2 (?f1 _) (?f2 _) ]
-                  => apply H
-                | [ H : forall x1 x2, ?R1 x1 x2 -> forall y1 y2, ?R2 y1 y2 -> ?R3 (?f1 x1 y1) (?f2 x2 y2) |- ?R3 (?f1 _ _) (?f2 _ _) ]
-                  => apply H
-                | [ H : forall x x', ?Rx x x' -> forall y y', _ -> forall z z', ?Rz z z' -> ?R (?f x y z) (?f' x' y' z') |- ?R (?f _ _ _) (?f' _ _ _) ]
-                  => apply H; clear H
-                | [ H : forall x x', _ -> forall y y', _ -> forall z z', _ -> forall w w', _ -> ?R (?f x y z w) (?f' x' y' z' w') |- ?R (?f _ _ _ _) (?f' _ _ _ _) ]
-                  => apply H; clear H
-                end
-              | progress cbv [Option.bind] in *
-              | match goal with
-                | [ H : expr.interp_related_gen _ _ ?e ?v |- _ ] => is_var e; clear H e
+                | [ |- context[match _ with nil => _ | _ => _ end] ] => progress recursive_match_to_case_in_goal
+                | [ |- context[match _ with pair a b => _ end] ] => progress recursive_match_to_case_in_goal
+                | [ |- context[match _ with true => _ | false => _ end] ] => progress recursive_match_to_case_in_goal
+                | [ |- context[match invert_expr.reflect_list ?ls with _ => _ end] ]
+                  => destruct (invert_expr.reflect_list ls) eqn:?
+                | [ |- context G[expr.interp_related_gen ?ident_interp (fun t : ?T => ?vii t ?b)] ]
+                  => progress change (fun t : T => vii t b) with (fun t : T => @Compile.value_interp_related _ ident_interp t b)
                 end ].
-
-      Local Ltac interp_good_t_step_arith :=
-        first [ lazymatch goal with
-                | [ |- ?x = ?x ] => reflexivity
-                | [ |- True ] => exact I
-                | [ H : ?x = true, H' : ?x = false |- _ ] => exfalso; clear -H H'; congruence
-                | [ H : true = false |- _ ]=> exfalso; clear -H; congruence
-                | [ H : false = true |- _ ]=> exfalso; clear -H; congruence
-                end
-              | progress cbv [option_beq] in *
-              | match goal with
-                | [ H : context[ZRange.normalize (ZRange.normalize _)] |- _ ]
-                  => rewrite ZRange.normalize_idempotent in H
-                | [ |- context[ZRange.normalize (ZRange.normalize _)] ]
-                  => rewrite ZRange.normalize_idempotent
-                | [ |- context[ident.cast (ZRange.normalize ?r)] ]
-                  => rewrite ident.cast_normalize
-                | [ H : context[ident.cast (ZRange.normalize ?r)] |- _ ]
-                  => rewrite ident.cast_normalize in H
-                | [ H : ?T, H' : ?T |- _ ] => clear H'
-                | [ H : context[is_bounded_by_bool _ (ZRange.normalize (-_))] |- _ ]
-                  => rewrite ZRange.is_bounded_by_bool_move_opp_normalize in H
-                | [ |- context[is_bounded_by_bool _ (ZRange.normalize (-_))] ]
-                  => rewrite ZRange.is_bounded_by_bool_move_opp_normalize
-                | [ H : is_bounded_by_bool ?v (ZRange.normalize ?r) = true |- context[ident.cast _ ?r ?v] ]
-                  => rewrite (@ident.cast_in_normalized_bounds _ r v) by exact H
-                | [ H : is_bounded_by_bool ?v (ZRange.normalize ?r) = true |- context[ident.cast _ (-?r) (-?v)] ]
-                  => rewrite (@ident.cast_in_normalized_bounds _ (-r) (-v));
-                     [ | clear -H ]
-                | [ |- context[ident.cast _ ?r (-ident.cast _ (-?r) ?v)] ]
-                  => rewrite (ident.cast_in_normalized_bounds r (-ident.cast _ (-r) v))
-                    by (rewrite <- ZRange.is_bounded_by_bool_move_opp_normalize; apply ident.cast_always_bounded)
-                | [ |- context[ident.cast _ ?r (ident.cast _ ?r _)] ]
-                  => rewrite (@ident.cast_idempotent _ _ r)
-                | [ H : is_bounded_by_bool _ ?r = true |- _]
-                  => is_var r; unique pose proof (ZRange.is_bounded_by_normalize _ _ H)
-                | [ H : lower ?x = upper ?x |- _ ] => is_var x; destruct x; cbn [upper lower] in *
-                | [ H : is_bounded_by_bool ?x (ZRange.normalize r[?y~>?y]) = true |- _ ]
-                  => apply ZRange.is_bounded_by_bool_normalize_constant_iff in H
-                | [ H : is_bounded_by_bool ?x r[?y~>?y] = true |- _ ]
-                  => apply ZRange.is_bounded_by_bool_constant_iff in H
-                end
-              | progress intros
-              | progress subst
-              | assumption
-              | progress destruct_head'_and
-              | progress Z.ltb_to_lt
-              | progress split_andb
-              | match goal with
-                | [ |- ?a mod ?b = ?a' mod ?b ] => apply f_equal2; lia
-                | [ |- ?a / ?b = ?a' / ?b ] => apply f_equal2; lia
-                | [ |- Z.opp _ = Z.opp _ ] => apply f_equal
-                end
-              | break_innermost_match_step
-              | break_innermost_match_hyps_step
-              | progress destruct_head'_or
-              | match goal with
-                | [ |- context[-ident.cast _ (-?r) (-?v)] ] => rewrite (ident.cast_opp' r v)
-                | [ |- context[ident.cast ?coor ?r ?v] ]
-                  => is_var v;
-                     pose proof (@ident.cast_always_bounded coor r v);
-                     generalize dependent (ident.cast coor r v); clear v; intro v; intros
-                | [ |- context[ident.cast ?coor ?r ?v] ]
-                  => is_var v; is_var coor;
-                     pose proof (@ident.cast_cases coor r v);
-                     generalize dependent (ident.cast coor r v); intros
-                | [ H : is_bounded_by_bool ?v ?r = true, H' : is_tighter_than_bool ?r ?r' = true |- _ ]
-                  => unique assert (is_bounded_by_bool v r' = true) by (eauto 2 using ZRange.is_bounded_by_of_is_tighter_than)
-                | [ H : is_bounded_by_bool (-?v) ?r = true, H' : (-?r <=? ?r')%zrange = true |- _ ]
-                  => unique assert (is_bounded_by_bool v r' = true)
-                    by (apply (@ZRange.is_bounded_by_of_is_tighter_than _ _ H');
-                        rewrite <- ZRange.is_bounded_by_bool_opp, ZRange.opp_involutive; exact H)
-                | [ H : is_bounded_by_bool ?v (-?r) = true |- _ ]
-                  => is_var v;
-                     unique assert (is_bounded_by_bool (-v) r = true)
-                       by now rewrite <- ZRange.is_bounded_by_bool_move_opp_normalize, ZRange.normalize_opp
-                | [ H : is_bounded_by_bool ?x r[0~>?v-1] = true |- _ ]
-                  => progress (try unique assert (0 <= x); try unique assert (x <= v - 1));
-                     [ clear -H; cbv [is_bounded_by_bool] in H; cbn [lower upper] in H; Bool.split_andb; Z.ltb_to_lt; lia..
-                     | ]
-                end
-              | progress cbn [expr.interp_related_gen] in *
-              | match goal with
-                | [ |- context[Z.shiftl] ] => rewrite Z.shiftl_mul_pow2 by auto with zarith
-                | [ |- context[Z.shiftr] ] => rewrite Z.shiftr_div_pow2 by auto with zarith
-                | [ |- context[Z.shiftl _ (-_)] ] => rewrite Z.shiftl_opp_r
-                | [ |- context[Z.land _ (Z.ones _)] ] => rewrite Z.land_ones by auto using Z.log2_nonneg
-                | [ |- context[- - _] ] => rewrite Z.opp_involutive
-                | [ H : ?x = 2^Z.log2 ?x |- context[2^Z.log2 ?x] ] => rewrite <- H
-                | [ H : ?x = 2^?n |- context[Z.land _ (?x - 1)] ]
-                  => rewrite !Z.sub_1_r, H, <- Z.ones_equiv, Z.land_ones by auto with zarith
-                | [ |- _ = _ :> BinInt.Z ] => progress normalize_commutative_identifier Z.land Z.land_comm
-                | [ H : ?x = ?y, H' : ?x <> ?y |- _ ] => exfalso; apply H', H
-                | [ H : ?x = 2^Z.log2_up ?x - 1 |- context[2^Z.log2_up ?x - 1] ] => rewrite <- H
-                | [ H : ?x = 2^Z.log2 ?x, H' : context[2^Z.log2 ?x] |- _ = _ :> BinInt.Z ]
-                  => rewrite <- H in H'
-                | [ |- _ = _ :> BinInt.Z ] => progress autorewrite with zsimplify_const
-                | [ H : 0 <= ?x, H' : ?x <= ?r - 1 |- context[?x mod ?r] ]
-                  => rewrite (Z.mod_small x r) by (clear -H H'; lia)
-                | [ H : 0 <= ?x, H' : ?x <= ?y - 1 |- context[?x / ?y] ]
-                  => rewrite (Z.div_small x y) by (clear -H H'; lia)
-                | [ H : ?x = 2^Z.log2 ?x |- _ ]
-                  => unique assert (0 <= x) by (rewrite H; auto with zarith)
-                | [ |- _ mod ?x = _ mod ?x ]
-                  => progress (push_Zmod; pull_Zmod)
-                | [ |- ?f (_ mod ?x) = ?f (_ mod ?x) ]
-                  => progress (push_Zmod; pull_Zmod)
-                | [ |- _ mod ?x = _ mod ?x ]
-                  => apply f_equal2; (lia + nia)
-                | _ => rewrite !Z.shiftl_mul_pow2 in * by auto using Z.log2_nonneg
-                | _ => rewrite !Z.land_ones in * by auto using Z.log2_nonneg
-                | H : ?x mod ?b * ?y <= _
-                  |- context [ (?x * ?y) mod ?b ] =>
-                  rewrite (PullPush.Z.mul_mod_l x y b);
-                  rewrite (Z.mod_small (x mod b * y) b) by omega
-                | [ |- context[_ - ?x + ?x] ] => rewrite !Z.sub_add
-                | [ |- context[_ mod (2^_) * 2^_] ] => rewrite <- !Z.mul_mod_distr_r_full
-                | [ |- context[Z.land _ (Z.ones _)] ] => rewrite !Z.land_ones by lia
-                | [ |- context[2^?a * 2^?b] ] => rewrite <- !Z.pow_add_r by lia
-                | [ |- context[-?x + ?y] ] => rewrite !Z.add_opp_l
-                | [ |- context[?n + - ?m] ] => rewrite !Z.add_opp_r
-                | [ |- context[?n - - ?m] ] => rewrite !Z.sub_opp_r
-                | [ |- context[Zpos ?p * ?x / Zpos ?p] ]
-                  => rewrite (@Z.div_mul' x (Zpos p)) in * by (clear; lia)
-                | [ H : context[Zpos ?p * ?x / Zpos ?p] |- _ ]
-                  => rewrite (@Z.div_mul' x (Zpos p)) in * by (clear; lia)
-                | [ |- ?f (?a mod ?r) = ?f (?b mod ?r) ] => apply f_equal; apply f_equal2; lia
-                | [ |- context[-?a - ?b + ?c] ] => replace (-a - b + c) with (c - a - b) by (clear; lia)
-                | [ |- context[?x - ?y + ?z] ]
-                  => lazymatch goal with
-                     | [ |- context[z - y + x] ]
-                       => progress replace (z - y + x) with (x - y + z) by (clear; lia)
-                     end
-                | [ |- context[?x - ?y - ?z] ]
-                  => lazymatch goal with
-                     | [ |- context[x - z - y] ]
-                       => progress replace (x - z - y) with (x - y - z) by (clear; lia)
-                     end
-                | [ |- context[?x + ?y] ]
-                  => lazymatch goal with
-                     | [ |- context[y + x] ]
-                       => progress replace (y + x) with (x + y) by (clear; lia)
-                     end
-                | [ |- context[?x + ?y + ?z] ]
-                  => lazymatch goal with
-                     | [ |- context[x + z + y] ]
-                       => progress replace (x + z + y) with (x + y + z) by (clear; lia)
-                     | [ |- context[z + x + y] ]
-                       => progress replace (z + x + y) with (x + y + z) by (clear; lia)
-                     | [ |- context[z + y + x] ]
-                       => progress replace (z + y + x) with (x + y + z) by (clear; lia)
-                     | [ |- context[y + x + z] ]
-                       => progress replace (y + x + z) with (x + y + z) by (clear; lia)
-                     | [ |- context[y + z + x] ]
-                       => progress replace (y + z + x) with (x + y + z) by (clear; lia)
-                     end
-                | [ |- - ident.cast _ (-?r) (- (?x / ?y)) = ident.cast _ ?r (?x' / ?y) ]
-                  => tryif constr_eq x x' then fail else replace x with x' by lia
-                | [ |- _ = _ :> BinInt.Z ] => progress autorewrite with zsimplify_fast
-                end ].
-
-      Local Ltac remove_casts :=
+      Local Ltac preprocess := repeat preprocess_step.
+      Local Ltac handle_extra_nbe :=
         repeat match goal with
-               | [ |- context[ident.cast _ ?r (ident.cast _ ?r _)] ]
-                 => rewrite ident.cast_idempotent
-               | [ H : context[ident.cast _ ?r (ident.cast _ ?r _)] |- _ ]
-                 => rewrite ident.cast_idempotent in H
-               | [ |- context[ident.cast ?coor ?r ?v] ]
-                 => is_var v;
-                    pose proof (@ident.cast_always_bounded coor r v);
-                    generalize dependent (ident.cast coor r v);
-                    clear v; intro v; intros
-               | [ H : context[ident.cast ?coor ?r ?v] |- _ ]
-                 => is_var v;
-                    pose proof (@ident.cast_always_bounded coor r v);
-                    generalize dependent (ident.cast coor r v);
-                    clear v; intro v; intros
-               | [ H : context[ZRange.constant ?v] |- _ ] => unique pose proof (ZRange.is_bounded_by_bool_normalize_constant v)
-               | [ H : is_tighter_than_bool (?ZRf ?r1 ?r2) (ZRange.normalize ?rs) = true,
-                       H1 : is_bounded_by_bool ?v1 ?r1 = true,
-                            H2 : is_bounded_by_bool ?v2 ?r2 = true
-                   |- _ ]
-                 => let cst := multimatch goal with
-                               | [ |- context[ident.cast ?coor rs (?Zf v1 v2)] ] => constr:(ident.cast coor rs (Zf v1 v2))
-                               | [ H : context[ident.cast ?coor rs (?Zf v1 v2)] |- _ ] => constr:(ident.cast coor rs (Zf v1 v2))
-                               end in
-                    lazymatch cst with
-                    | ident.cast ?coor rs (?Zf v1 v2)
-                      => let lem := lazymatch constr:((ZRf, Zf)%core) with
-                                    | (ZRange.shiftl, Z.shiftl)%core => constr:(@ZRange.is_bounded_by_bool_shiftl v1 r1 v2 r2 H1 H2)
-                                    | (ZRange.shiftr, Z.shiftr)%core => constr:(@ZRange.is_bounded_by_bool_shiftr v1 r1 v2 r2 H1 H2)
-                                    | (ZRange.land, Z.land)%core => constr:(@ZRange.is_bounded_by_bool_land v1 r1 v2 r2 H1 H2)
-                                    end in
-                         try unique pose proof (@ZRange.is_bounded_by_of_is_tighter_than _ _ H _ lem);
-                         clear H;
-                         rewrite (@ident.cast_in_normalized_bounds coor rs (Zf v1 v2)) in * by assumption
-                    end
-               | [ H : is_tighter_than_bool (?ZRf ?r1) (ZRange.normalize ?rs) = true,
-                       H1 : is_bounded_by_bool ?v1 ?r1 = true
-                   |- _ ]
-                 => let cst := multimatch goal with
-                               | [ |- context[ident.cast ?coor rs (?Zf v1)] ] => constr:(ident.cast coor rs (Zf v1))
-                               | [ H : context[ident.cast ?coor rs (?Zf v1)] |- _ ] => constr:(ident.cast coor rs (Zf v1))
-                               end in
-                    lazymatch cst with
-                    | ident.cast ?coor rs (?Zf v1)
-                      => let lem := lazymatch constr:((ZRf, Zf)%core) with
-                                    | (ZRange.cc_m ?s, Z.cc_m ?s)%core => constr:(@ZRange.is_bounded_by_bool_cc_m s v1 r1 H1)
-                                    end in
-                         try unique pose proof (@ZRange.is_bounded_by_of_is_tighter_than _ _ H _ lem);
-                         clear H;
-                         rewrite (@ident.cast_in_normalized_bounds coor rs (Zf v1)) in * by assumption
-                    end
-               | [ H : is_bounded_by_bool ?v (ZRange.normalize ?r) = true |- context[ident.cast ?coor ?r ?v] ]
-                 => rewrite (@ident.cast_in_normalized_bounds coor r v) in * by assumption
-               | [ H : is_bounded_by_bool ?v (ZRange.normalize ?r) = true, H' : context[ident.cast ?coor ?r ?v] |- _ ]
-                 => rewrite (@ident.cast_in_normalized_bounds coor r v) in * by assumption
-               | [ H : is_bounded_by_bool ?v ?r = true,
-                       H' : is_tighter_than_bool ?r r[0~>?x-1]%zrange = true,
-                            H'' : Z.eqb ?x ?m = true
-                   |- context[?v mod ?m] ]
-                 => unique assert (is_bounded_by_bool v r[0~>x-1] = true)
-                   by (eapply ZRange.is_bounded_by_of_is_tighter_than; eassumption)
-               | _ => progress Z.ltb_to_lt
-               | _ => progress subst
+               | [ |- UnderLets.interp_related _ _ (UnderLets.Base (expr.Ident _)) _ ]
+                 => cbn [UnderLets.interp_related UnderLets.interp_related_gen expr.interp_related_gen ident_interp type.related]; reflexivity
+               | [ |- UnderLets.interp_related _ _ (UnderLets.Base (reify_list _)) _ ]
+                 => cbn [UnderLets.interp_related UnderLets.interp_related_gen]; rewrite expr.reify_list_interp_related_gen_iff
+               | [ |- UnderLets.interp_related _ _ (UnderLets.Base (_, _)%expr) ?x ]
+                 => cbn [UnderLets.interp_related UnderLets.interp_related_gen];
+                    recurse_interp_related_step;
+                    [ recurse_interp_related_step
+                    | lazymatch x with
+                      | (_, _) => reflexivity
+                      | _ => etransitivity; [ | symmetry; apply surjective_pairing ]; reflexivity
+                      end ];
+                    [ | reflexivity ]; cbn [fst snd];
+                    recurse_interp_related_step; [ recurse_interp_related_step | reflexivity ]
+               | [ |- List.Forall2 _ (List.map _ _) _ ]
+                 => rewrite Forall2_map_l_iff
+               | [ |- List.Forall2 _ ?x ?x ] => rewrite Forall2_Forall; cbv [Proper]
+               | [ |- List.Forall _ _ ] => rewrite Forall_forall; intros
+               | [ |- expr.interp_related_gen _ _ (expr.Ident _) _ ]
+                 => cbn [expr.interp_related_gen ident_interp type.related]; reflexivity
                end.
+      Local Ltac fin_tac :=
+        repeat first [ assumption
+                     | progress change S with Nat.succ
+                     | progress cbn [base.interp base.base_interp type.interp] in *
+                     | progress fold (@type.interp _ base.interp)
+                     | progress fold (@base.interp)
+                     | progress subst
+                     | progress cbv [respectful ident.Thunked.bool_rect ident.Thunked.list_case ident.Thunked.option_rect pointwise_relation]
+                     | progress intros
+                     | solve [ auto ]
+                     | match goal with
+                       | [ |- ?x = ?x ] => reflexivity
+                       | [ |- list_rect _ _ _ _ = ident.Thunked.list_rect _ _ _ _ ]
+                         => cbv [ident.Thunked.list_rect]; apply list_rect_Proper; cbv [pointwise_relation]; intros
+                       | [ |- list_rect (fun _ => ?A -> ?B) _ _ _ _ = list_rect _ _ _ _ _ ]
+                         => apply list_rect_arrow_Proper; cbv [respectful]; intros
+                       | [ |- nat_rect _ _ _ _ = ident.Thunked.nat_rect _ _ _ _ ]
+                         => apply nat_rect_Proper_nondep; cbv [respectful]
+                       | [ |- nat_rect (fun _ => ?A -> ?B) _ _ _ _ = nat_rect _ _ _ _ _ ]
+                         => apply (@nat_rect_Proper_nondep_gen (A -> B) (eq ==> eq)%signature); cbv [respectful]; intros
+                       | [ |- list_case _ _ _ ?ls = list_case _ _ _ ?ls ]
+                         => is_var ls; destruct ls; cbn [list_case]
+                       | [ |- bool_rect _ _ _ ?b = bool_rect _ _ _ ?b ]
+                         => is_var b; destruct b; cbn [bool_rect]
+                       | [ |- _ = ident.cast2 _ _ _ ] => cbv [ident.cast2]; break_innermost_match
+                       end ].
+      Local Ltac handle_reified_rewrite_rules_interp :=
+        repeat first [ assumption
+                     | match goal with
+                       | [ |- UnderLets.interp_related _ _ (Reify.expr_value_to_rewrite_rule_replacement _ ?sda _) _ ]
+                         => apply (@Reify.expr_value_to_rewrite_rule_replacement_interp_related cast_outside_of_range _ (@Reify.reflect_ident_iota_interp_related cast_outside_of_range) sda)
 
-      Local Ltac unfold_cast_lemmas :=
-        repeat match goal with
-               | [ H : context[ZRange.normalize (ZRange.constant _)] |- _ ]
-                 => rewrite ZRange.normalize_constant in H
-               | [ H : is_bounded_by_bool _ (ZRange.normalize ?r) = true |- _ ]
-                 => is_var r; generalize dependent (ZRange.normalize r); clear r; intro r; intros
-               | [ H : is_bounded_by_bool ?x (ZRange.constant ?x) = true |- _ ]
-                 => clear H
-               | [ H : is_bounded_by_bool ?x ?r = true |- _ ]
-                 => is_var r; apply unfold_is_bounded_by_bool in H
-               | [ H : is_bounded_by_bool ?x r[_~>_] = true |- _ ]
-                 => apply unfold_is_bounded_by_bool in H
-               | [ H : is_tighter_than_bool r[_~>_] r[_~>_] = true |- _ ]
-                 => apply unfold_is_tighter_than_bool in H
-               | _ => progress cbn [lower upper] in *
-               | [ H : context[lower ?r] |- _ ]
-                 => is_var r; let l := fresh "l" in let u := fresh "u" in destruct r as [l u]
-               | [ H : context[upper ?r] |- _ ]
-                 => is_var r; let l := fresh "l" in let u := fresh "u" in destruct r as [l u]
-               | _ => progress Z.ltb_to_lt
-               end.
+                       | [ |- UnderLets.interp_related_gen ?ii ?R (UnderLets.Base (#ident.list_rect @ _ @ _ @ _)%expr) (@list_rect ?A (fun _ => ?P) ?N ?C ?ls) ]
+                         => progress change (@list_rect A (fun _ => P) N C ls) with (@ident.Thunked.list_rect A P (fun _ => N) C ls)
+                       | [ |- expr.interp_related_gen ?ii ?R (#ident.list_rect @ _ @ _ @ _)%expr (@list_rect ?A (fun _ => ?P) ?N ?C ?ls) ]
+                         => progress change (@list_rect A (fun _ => P) N C ls) with (@ident.Thunked.list_rect A P (fun _ => N) C ls)
+                       | [ |- expr.interp_related_gen ?ii ?R (#ident.eager_list_rect @ _ @ _ @ _)%expr (@list_rect ?A (fun _ => ?P) ?N ?C ?ls) ]
+                         => progress change (@list_rect A (fun _ => P) N C ls) with (@ident.Thunked.list_rect A P (fun _ => N) C ls)
+                       | [ |- expr.interp_related_gen ?ii ?R (#ident.list_case @ _ @ _ @ _)%expr (@list_case ?A (fun _ => ?P) ?N ?C ?ls) ]
+                         => progress change (@list_case A (fun _ => P) N C ls) with (@ident.Thunked.list_case A P (fun _ => N) C ls)
+                       | [ |- expr.interp_related_gen ?ii ?R (#ident.nat_rect @ _ @ _ @ _)%expr (@nat_rect (fun _ => ?P) ?N ?C ?ls) ]
+                         => progress change (@nat_rect (fun _ => P) N C ls) with (@ident.Thunked.nat_rect P (fun _ => N) C ls)
+                       | [ |- expr.interp_related_gen ?ii ?R (#ident.eager_nat_rect @ _ @ _ @ _)%expr (@nat_rect (fun _ => ?P) ?N ?C ?ls) ]
+                         => progress change (@nat_rect (fun _ => P) N C ls) with (@ident.Thunked.nat_rect P (fun _ => N) C ls)
+                       | [ |- expr.interp_related_gen ?ii ?R (#ident.bool_rect @ _ @ _ @ _)%expr (@bool_rect (fun _ => ?P) ?T ?F ?b) ]
+                         => progress change (@bool_rect (fun _ => P) T F b) with (@ident.Thunked.bool_rect P (fun _ => T) (fun _ => F) b)
+                       | [ |- expr.interp_related_gen ?ii ?R (#ident.option_rect @ _ @ _ @ _)%expr (@option_rect ?A (fun _ => ?P) ?S ?N ?o) ]
+                         => progress change (@option_rect A (fun _ => P) S N o) with (@ident.Thunked.option_rect A P S (fun _ => N) o)
 
-      Local Ltac systematically_handle_casts :=
-        remove_casts; unfold_cast_lemmas.
+                       | [ |- match ?x with pair _ _ => _ end = prod_rect _ _ _ ]
+                         => cbv [prod_rect]; eta_expand
 
-      Local Ltac fin_with_nia :=
-        lazymatch goal with
-        | [ |- ident.cast _ ?r _ = ident.cast _ ?r _ ] => apply f_equal; Z.div_mod_to_quot_rem; nia
-        | _ => reflexivity || (Z.div_mod_to_quot_rem; (lia + nia))
-        end.
+                       | [ |- expr.interp_related_gen _ _ (expr.Var _) _ ]
+                         => cbn [expr.interp_related_gen]
+                       | [ |- expr.interp_related_gen _ _ (expr.Ident _) _ ]
+                         => cbn [expr.interp_related_gen ident_interp type.related]; fin_tac
+                       | [ |- expr.interp_related_gen _ _ (expr.Abs ?f) _ ]
+                         => let fh := fresh in set (fh := f); cbn [expr.interp_related_gen]; subst fh; cbv beta; intros
+                       | [ |- expr.interp_related_gen _ _ (expr.LetIn ?v ?f) (LetIn.Let_In ?V ?F) ]
+                         => let vh := fresh in
+                            set (vh := v);
+                            let fh := fresh in
+                            set (fh := f);
+                            cbn [expr.interp_related_gen]; subst fh vh; cbv beta;
+                            exists F, V; repeat apply conj; intros
+                       | [ |- expr.interp_related_gen _ _ (?f @ ?x)%expr (?F ?X) ]
+                         => let fh := fresh in
+                            set (fh := f);
+                            let xh := fresh in
+                            set (xh := x);
+                            cbn [expr.interp_related_gen]; subst fh xh;
+                            exists F, X; repeat apply conj; [ | | reflexivity ]
 
-      Lemma nbe_rewrite_rules_interp_good
-        : rewrite_rules_interp_goodT nbe_rewrite_rules.
+                       | [ |- _ = _ ] => solve [ fin_tac ]
+                       end ].
+
+
+      Local Notation specT rewriter_data
+        := (PrimitiveHList.hlist (@snd bool Prop) (List.skipn (dummy_count rewriter_data) (rewrite_rules_specs rewriter_data)))
+             (only parsing).
+
+      Lemma nbe_rewrite_rules_interp_good (H : specT nbe_rewriter_data)
+        : rewrite_rules_interp_goodT (rewrite_rules nbe_rewriter_data _).
       Proof using Type.
         Time start_interp_good.
-        Time all: try solve [ repeat interp_good_t_step_related ].
-      Qed.
+        Time all: preprocess; handle_extra_nbe; handle_reified_rewrite_rules_interp.
+      Time Qed.
 
-      Lemma arith_rewrite_rules_interp_good max_const
-        : rewrite_rules_interp_goodT (arith_rewrite_rules max_const).
+      Lemma arith_rewrite_rules_interp_good max_const (H : specT (arith_rewriter_data max_const))
+        : rewrite_rules_interp_goodT (rewrite_rules (arith_rewriter_data max_const) _).
       Proof using Type.
         Time start_interp_good.
-        Time all: try solve [ repeat interp_good_t_step_related; repeat interp_good_t_step_arith; fin_with_nia ].
-      Qed.
+        Time all: preprocess; handle_reified_rewrite_rules_interp.
+      Time Qed.
 
-      Lemma arith_with_casts_rewrite_rules_interp_good
-        : rewrite_rules_interp_goodT arith_with_casts_rewrite_rules.
+      Lemma arith_with_casts_rewrite_rules_interp_good (H : specT arith_with_casts_rewriter_data)
+        : rewrite_rules_interp_goodT (rewrite_rules arith_with_casts_rewriter_data _).
       Proof using Type.
         Time start_interp_good.
-        Time all: try solve [ repeat interp_good_t_step_related; repeat interp_good_t_step_arith; fin_with_nia ].
-      Qed.
+        Time all: preprocess; handle_reified_rewrite_rules_interp.
+      Time Qed.
 
-      Lemma strip_literal_casts_rewrite_rules_interp_good
-        : rewrite_rules_interp_goodT strip_literal_casts_rewrite_rules.
+      Lemma strip_literal_casts_rewrite_rules_interp_good (H : specT strip_literal_casts_rewriter_data)
+        : rewrite_rules_interp_goodT (rewrite_rules strip_literal_casts_rewriter_data _).
       Proof using Type.
         Time start_interp_good.
-        Time all: try solve [ repeat interp_good_t_step_related; repeat interp_good_t_step_arith ].
-      Qed.
-
-      Local Ltac fancy_local_t :=
-        repeat match goal with
-               | [ H : forall s v v', ?invert_low s v = Some v' -> v = _,
-                     H' : ?invert_low _ _ = Some _ |- _ ] => apply H in H'
-               | [ H : forall s v v', ?invert_low s v = Some v' -> v = _ |- _ ]
-                 => clear invert_low H
-               end.
-      Local Ltac more_fancy_arith_t := repeat autorewrite with zsimplify in *.
+        Time all: preprocess; handle_reified_rewrite_rules_interp.
+      Time Qed.
 
       Lemma fancy_rewrite_rules_interp_good
             (invert_low invert_high : Z -> Z -> option Z)
             (Hlow : forall s v v', invert_low s v = Some v' -> v = Z.land v' (2^(s/2)-1))
             (Hhigh : forall s v v', invert_high s v = Some v' -> v = Z.shiftr v' (s/2))
-        : rewrite_rules_interp_goodT fancy_rewrite_rules.
+            (H : specT (fancy_rewriter_data invert_low invert_high))
+        : rewrite_rules_interp_goodT (rewrite_rules (fancy_rewriter_data invert_low invert_high) _).
       Proof using Type.
         Time start_interp_good.
-        Time all: try solve [ repeat interp_good_t_step_related ].
-      Qed.
+        Time all: preprocess; handle_reified_rewrite_rules_interp.
+      Time Qed.
 
       Lemma fancy_with_casts_rewrite_rules_interp_good
             (invert_low invert_high : Z -> Z -> option Z)
             (value_range flag_range : zrange)
             (Hlow : forall s v v', invert_low s v = Some v' -> v = Z.land v' (2^(s/2)-1))
             (Hhigh : forall s v v', invert_high s v = Some v' -> v = Z.shiftr v' (s/2))
-        : rewrite_rules_interp_goodT (fancy_with_casts_rewrite_rules invert_low invert_high value_range flag_range).
+            (H : specT (fancy_with_casts_rewriter_data invert_low invert_high value_range flag_range))
+        : rewrite_rules_interp_goodT (rewrite_rules (fancy_with_casts_rewriter_data invert_low invert_high value_range flag_range) _).
       Proof using Type.
-        Time start_interp_good. (* Finished transaction in 1.206 secs (1.207u,0.s) (successful) *)
-        Set Ltac Profiling.
-        Reset Ltac Profile.
-        Time all: repeat interp_good_t_step_related. (* Finished transaction in 13.259 secs (13.128u,0.132s) (successful) *)
-        Reset Ltac Profile.
-        Time all: fancy_local_t. (* Finished transaction in 0.051 secs (0.052u,0.s) (successful) *)
-        Time all: systematically_handle_casts. (* Finished transaction in 2.004 secs (1.952u,0.052s) (successful) *)
-        Time all: try solve [ repeat interp_good_t_step_arith ]. (* Finished transaction in 44.411 secs (44.004u,0.411s) (successful) *)
-      Qed.
+        Time start_interp_good.
+        Time all: preprocess; handle_reified_rewrite_rules_interp.
+      Time Qed.
     End with_cast.
   End RewriteRules.
 End Compilers.
